

1 Proof the MSNE is a CE

Say that $\sigma^* = (\sigma_i^*, \sigma_{-i}^*)$ is a MSNE of an SFG. Then according to definition 6 of MSNE in lectures 12 to 15, for all $i \in N$,

$$\begin{aligned} U_i(s_i, \sigma_{-i}^*) & \text{ is same for all } s_i \in \delta(\sigma_i^*) \\ U_i(s_i, \sigma_{-i}^*) & \geq U_i(s_i', \sigma_{-i}^*), \forall s_i \in \delta(\sigma_i^*), s_i' \notin \delta(\sigma_i^*) \end{aligned}$$

Writting the above two equations in expanded form we get,

$$\sum_{s_{-i}} \sigma_{-i}^*(s_{-i}) u_i(s_i, s_{-i}) = \sum_{s_{-i}} \sigma_{-i}^*(s_{-i}) u_i(s_i', s_{-i}), \forall s_i \in \delta(\sigma_i^*), s_i' \in \delta(\sigma_i^*), \forall i \in N \quad (1)$$

$$\sum_{s_{-i}} \sigma_{-i}^*(s_{-i}) u_i(s_i, s_{-i}) \geq \sum_{s_{-i}} \sigma_{-i}^*(s_{-i}) u_i(s_i', s_{-i}), \forall s_i \in \delta(\sigma_i^*), s_i' \notin \delta(\sigma_i^*), \forall i \in N \quad (2)$$

Equations (1) and (2) implies,

$$\sum_{s_{-i}} \sigma_{-i}^*(s_{-i}) u_i(s_i, s_{-i}) \geq \sum_{s_{-i}} \sigma_{-i}^*(s_{-i}) u_i(s_i', s_{-i}), \forall s_i \in \delta(\sigma_i^*), s_i' \in S_i, \forall i \in N \quad (3)$$

We want to prove that if we set

$$\sigma(s_i, s_{-i}) = \sigma_i^*(s_i) \sigma_{-i}^*(s_{-i}), \forall s_i \in S_i, s_{-i} \in S_{-i}, \forall i \in N \quad (4)$$

then $\sigma(s_i, s_{-i})$ will be a CE. In other words $\sigma(s_i, s_{-i})$ given by equation (4) will satisfy,

$$\sum_{s_{-i}} \sigma(s_i, s_{-i}) u_i(s_i, s_{-i}) \geq \sum_{s_{-i}} \sigma(s_i, s_{-i}) u_i(s_i', s_{-i}), \forall s_i, s_i' \in S_i, \forall i \in N$$

So essentially, we want to prove that,

$$\sum_{s_{-i}} \sigma_i^*(s_i) \sigma_{-i}^*(s_{-i}) u_i(s_i, s_{-i}) \geq \sum_{s_{-i}} \sigma_i^*(s_i) \sigma_{-i}^*(s_{-i}) u_i(s_i', s_{-i}), \forall s_i, s_i' \in S_i, \forall i \in N \quad (5)$$

We divide the proof into two cases.

CASE-1 ($s_i \notin \delta(\sigma_i^*)$):

Since $s_i \notin \delta(\sigma_i^*)$, then by definition $\sigma_i^*(s_i) = 0$. In this case, both LHS and RHS of inequality (5) are zero and hence inequality (5) is true.

CASE-2 ($s_i \in \delta(\sigma_i^*)$):

Consider the LHS of inequality (5). We have,

$$\begin{aligned} \sum_{s_{-i}} \sigma_i^*(s_i) \sigma_{-i}^*(s_{-i}) u_i(s_i, s_{-i}) &= \sigma_i^*(s_i) \sum_{s_{-i}} \sigma_{-i}^*(s_{-i}) u_i(s_i, s_{-i}) \\ &\geq \sigma_i^*(s_i) \sum_{s_{-i}} \sigma_{-i}^*(s_{-i}) u_i(s_i', s_{-i}) \quad \text{using (3)} \\ &= \sum_{s_{-i}} \sigma_i^*(s_i) \sigma_{-i}^*(s_{-i}) u_i(s_i', s_{-i}) \end{aligned} \quad (6)$$

This concludes the proof.